src/lib/data/Kuiper.Index.fsti
@@ -3,6 +3,7 @@ module Kuiper.Index
 open Kuiper.Bijection
 open Kuiper.Common
 open Kuiper.SizeT
+module SZ = Kuiper.SizeT
 
 (* An idesc represents a tensor type, where every ICons adds a dimension.
    MxN matrix = ICons m (ICons n INil) *)
@@ -10,15 +11,29 @@ open Kuiper.SizeT
 noeq
 type idesc : nat -> Type =
   | INil : idesc 0
-  | ICons : #n:nat -> w:nat{SizeT.fits w} -> tl:(idesc n) -> idesc (n+1)
+  | ICons : #n:nat -> w:nat -> tl:(idesc n) -> idesc (n+1)
+
+let tail (#n:pos) (d : idesc n) : idesc (n-1) =
+  match d with
+  | ICons _ tl -> tl
 
 [@@strict_on_arguments [1]]
-let rec ( @! ) (#n:nat) (d : idesc n) (i : natlt n) : GTot (x:nat{SizeT.fits x}) =
+let rec ( @! ) (#n:nat) (d : idesc n) (i : natlt n) : GTot nat =
   match d with
   | ICons t ts ->
     match i with
     | 0 -> t
     | i -> ts @! (i - 1)
+
+#push-options "--warn_error -271"
+let rec lemma_at_tail (#n:nat) (d : idesc n) (i : natlt (n-1))
+  : Lemma (d @! (i+1) == tail d @! i)
+  = match d with
+    | ICons t ts ->
+      match i with
+      | 0 -> ()
+      | i -> lemma_at_tail ts (i - 1)
+#pop-options
 
 [@@strict_on_arguments [1]]
 let rec sizeof (#r : nat) (d : idesc r) : GTot nat =
@@ -47,36 +62,77 @@ let rec up #n (#d : idesc n) (v : conc d) : GTot (abs d) =
   | INil -> ()
   | ICons t ts ->
     let i1, is = v <: szlt t & conc ts in
-    ((FStar.SizeT.v i1 <: natlt t), up is)
+    ((SZ.v i1 <: natlt t), up is)
+
+let rec all_fit (#n:nat) (d : idesc n) : prop =
+  match d with
+  | INil -> True
+  | ICons t ts -> SZ.fits t /\ all_fit ts
+
+let all_fit' (#n:nat) (d : idesc n) : prop =
+  forall (i : natlt n). SZ.fits (d @! i)
+
+let rec all_fit_iff_all_fit' (#n:nat) (d : idesc n) : Lemma (all_fit d <==> all_fit' d)
+        [SMTPat (all_fit d)]
+  = match d with
+    | INil -> ()
+    | ICons t ts ->
+      calc (<==>) {
+        all_fit (ICons t ts);
+        <==> {}
+        SZ.fits t /\ all_fit ts;
+        <==> { all_fit_iff_all_fit' ts }
+        SZ.fits t /\ (forall (i : natlt (n-1)). SZ.fits (ts @! i));
+        <==> {}
+        SZ.fits (d @! 0) /\ (forall (i : natlt (n-1)). SZ.fits (tail d @! i));
+        <==> { Classical.forall_intro (lemma_at_tail d) }
+        (forall (i : natlt n). SZ.fits (ICons t ts @! i));
+      };
+      ()
 
 [@@strict_on_arguments [1]]
-let rec down #n (#d : idesc n) (v : abs d) : GTot (conc d) =
+let rec down #n (#d : idesc n{all_fit d}) (v : abs d) : GTot (conc d) =
   match d with
   | INil -> ()
   | ICons t ts ->
     let i1, is = v <: natlt t & abs ts in
-    ((FStar.SizeT.uint_to_t i1 <: szlt t), down is)
+    ((SZ.uint_to_t i1 <: szlt t), down is)
 
+// The refinement on v (which talks about d....) seems to be better than having
+// a precondition on the lemma, otherwise the trigger does not seem to work.  A
+// refinement on d itself, or squash arguments, also fail to trigger.
 val up_down #n (#d : idesc n) (v : abs d) :
-  Lemma (up (down v) == v)
+  Lemma (ensures all_fit d ==> up (down v) == v)
         [SMTPat (up (down v))]
 
 val down_up #n (#d : idesc n) (v : conc d) :
-  Lemma (down (up v) == v)
+  Lemma (ensures all_fit d ==> down (up v) == v)
         [SMTPat (down (up v))]
 
 (* Remove (fix) a given dimension *)
 let rec modulo_i (#n:nat) (i : natlt n) (d : idesc n) : idesc (n-1) =
   (* Cannot match on d and i simultaneously *)
   match d with
-  | INil -> assert False; INil
   | ICons t ts ->
     match i with
     | 0 -> ts
     | i -> ICons t (modulo_i (i-1) ts)
 
+#push-options "--warn_error -271"
+let rec all_fit_modulo (#n:nat) (i : natlt n) (d : idesc n)
+  : Lemma (requires all_fit d)
+          (ensures  all_fit (modulo_i i d))
+          [SMTPat (all_fit d); SMTPat (all_fit (modulo_i i d))]
+  = match d with
+    | INil -> ()
+    | ICons t ts ->
+      match i with
+      | 0 -> ()
+      | i -> all_fit_modulo (i-1) ts
+#pop-options
+
 (* Insert a dimension. Note the n+1, one can insert at the very end. *)
-let rec insert_i (#n:nat) (i : natlt (n+1)) (k : nat{SizeT.fits k}) (d : idesc n) : idesc (n+1) =
+let rec insert_i (#n:nat) (i : natlt (n+1)) (k : nat) (d : idesc n) : idesc (n+1) =
   match i with
   | 0 -> ICons k d
   | i -> ICons (d @! 0) (insert_i (i-1) k (modulo_i 0 d))
@@ -88,7 +144,7 @@ val insert_modulo (#n:nat) (i : natlt n) (d : idesc n)
   : Lemma (insert_i #(n-1) i (d @! i) (modulo_i i d) == d)
           [SMTPat (insert_i #(n-1) i (d @! i) (modulo_i i d))]
 
-val modulo_insert (#n:nat) (i : natlt (n+1)) (k : nat{SizeT.fits k}) (d : idesc n)
+val modulo_insert (#n:nat) (i : natlt (n+1)) (k : nat{SZ.fits k}) (d : idesc n)
   : Lemma (ensures modulo_i i (insert_i i k d) == d)
           [SMTPat (modulo_i i (insert_i i k d))]
 
@@ -96,7 +152,7 @@ val modulo_size_lemma (#n:nat) (i : natlt n) (d : idesc n)
   : Lemma (sizeof (modulo_i i d) * (d @! i) == sizeof d)
           [SMTPat (sizeof (modulo_i i d)); SMTPat (sizeof d)]
 
-val insert_size_lemma (#n:nat) (i : natlt (n+1)) (k : nat{SizeT.fits k}) (d : idesc n)
+val insert_size_lemma (#n:nat) (i : natlt (n+1)) (k : nat{SZ.fits k}) (d : idesc n)
   : Lemma (sizeof (insert_i i k d) == sizeof d * k)
           [SMTPat (sizeof (insert_i i k d)); SMTPat (sizeof d)]
 #pop-options
@@ -106,7 +162,7 @@ let rec abs_bring_forward_bij (#n:nat) (i : natlt n) (d : idesc n)
   = match i with
     | 0 -> bij_self _
     | _ ->
-      bij_prod (bij_self _) (abs_bring_forward_bij (i-1) (ICons?.tl d))
+      bij_prod (bij_self _) (abs_bring_forward_bij (i-1) (tail d))
       `bij_comp`
       bij_push_tuple3 #(natlt (d @! 0))
 
@@ -139,13 +195,14 @@ let rec c_conc_bring_forward_bij (#n : Ghost.erased nat) (i : szlt n) (d : idesc
     v                                         v
    conc d --conc_bring_forward--> szlt (d @! i) & conc (modulo_i i d)
 *)
-let down2 (#n:nat) (i : natlt n) (d : idesc n)
+let down2 (#n:nat) (i : natlt n) (d : idesc n{all_fit d})
   (tup : natlt (d @! i) & abs (modulo_i i d))
   : GTot (szlt (d @! i) & conc (modulo_i i d))
   = match tup with
-    | (j, abs_mod) -> ((FStar.SizeT.uint_to_t j <: szlt (d @! i)), down abs_mod)
+    | (j, abs_mod) ->
+      ((SZ.uint_to_t j <: szlt (d @! i)), down abs_mod)
 
-val bring_forward_commute (#n:nat) (i : natlt n) (d : idesc n)
+val bring_forward_commute (#n:nat) (i : natlt n) (d : idesc n{all_fit d})
   (idx : abs d)
   : Lemma (down2 i d ((abs_bring_forward_bij i d).ff idx) ==
           (conc_bring_forward_bij i d).ff (down idx))
@@ -153,13 +210,14 @@ val bring_forward_commute (#n:nat) (i : natlt n) (d : idesc n)
 val bring_forward_commute2 (#n:nat) (i : natlt n) (d : idesc n)
   (j : szlt (d @! i)) (idx : conc (modulo_i i d))
   : Lemma (up ((conc_bring_forward_bij i d).gg (j, idx))
-           == (abs_bring_forward_bij i d).gg (SizeT.v j, up idx))
+           == (abs_bring_forward_bij i d).gg (SZ.v j, up idx))
 
-let abs_conc_bij (#n:nat) (d : idesc n)
+// This bijection only exists when all_fit holds.
+let abs_conc_bij (#n:nat) (d : idesc n{all_fit d})
   : (abs d =~ conc d)
   = {
     ff = down;
     gg = up;
-    ff_gg = (fun v -> down_up v);
-    gg_ff = (fun v -> up_down v);
+    ff_gg = (fun (v : conc d) -> down_up v);
+    gg_ff = (fun (v : abs d) -> up_down v);
   }
